Never mind

src/simple-proof/proof/Congruence.v
@@ -22,7 +22,7 @@ Fixpoint congruence (e : ec) (t : trm) (k : nat) : (option (ec * trm)) :=
       match t with
       | trm_val v =>
         let x := (var_gen (dom s)) in
-        congruence (e_hole (s & x ~ v)) (open_trm x t) n
+        congruence (e_hole (s & x ~ v)) (open_trm x u) n
       | _ => Some (e, t)
       end
     end
@@ -37,13 +37,13 @@ Inductive red_congruence : ec -> trm -> ec -> trm -> Prop :=
     let x := (var_gen (dom s)) in
     red_congruence (e_term s t) (trm_val v) (e_hole (s & (x ~ v))) (open_trm x t).
 
-Lemma congruence_deterministic: forall e t e' t' e'' t'',
-    red_congruence e t e' t' ->
-    red_congruence e t e'' t'' ->
-    e' = e'' /\ t' = t''.
-Proof.
-  intros. inversions H; inversions H0; auto.
-Qed.
+Inductive red_congruence_closure : ec -> trm -> ec -> trm -> Prop :=
+| closure_refl : forall e t,
+    red_congruence_closure e t e t
+| closure_step: forall e t e' t' e'' t'',
+    red_congruence_closure e t e' t' ->
+    red_congruence e' t' e'' t'' ->
+    red_congruence_closure e t e'' t''.
 
 Fixpoint double_num_lets (t : trm) : nat :=
   match t with
@@ -57,13 +57,51 @@ Definition double_num_lets_pair (e : ec) (t : trm) : nat :=
   | e_term _ u => 2 + (double_num_lets t) + (double_num_lets u)
   end.
 
+Lemma congruence_fixpoint_relation_equiv : forall e t e' t',
+    congruence e t (double_num_lets_pair e t) = Some (e', t') ->
+    red_congruence_closure e t e' t'.
+Proof.
+  intros. induction t; induction e; simpl in *; try solve [inversions H].
+  - inversions H. apply closure_refl.
+  - induction t; inversions H.
+    + apply closure_step with (e':=e_term s (trm_var a)) (t':=trm_val v).
+      * apply closure_refl.
+      * apply red_congruence_val'.
+    + apply closure_step with (e':=e_term s (trm_val v0)) (t':=trm_val v).
+      * apply closure_refl.
+      * apply red_congruence_val'.
+    + apply closure_step with (e':=e_term s (trm_sel a t)) (t':=trm_val v).
+      * apply closure_refl.
+      * apply red_congruence_val'.
+    + apply closure_step with (e':=e_term s (trm_app a a0)) (t':=trm_val v).
+      * apply closure_refl.
+      * apply red_congruence_val'.
+    +
+
+Qed.
+ (* inversions H. apply closure_step with (e':=(e_term s t)) (t':=(trm_val v)). *)
+ (*    + apply closure_refl. *)
+ (*    +  *)Admitted.
+
+Lemma congruence_deterministic: forall e t e' t' e'' t'',
+    red_congruence e t e' t' ->
+    red_congruence e t e'' t'' ->
+    e' = e'' /\ t' = t''.
+Proof.
+  intros. inversions H; inversions H0; auto.
+Qed.
+
 Lemma congruence_max: forall e t e' t' e'' t'',
     congruence e t (double_num_lets_pair e t) = Some (e', t') ->
     red_congruence e' t' e'' t'' ->
     False.
 Proof.
   intros. destruct t; destruct e; simpl in *; try solve [inversions H; inversions H0].
+  - gen s v e' t'.
+    induction t; intros; try solve [inversions H; inversions H0].
+    simpl in *. induction t1; try solve [inversions H; inversions H0].
+    simpl in *. inversions H0. inversions H.
   - destruct (double_num_lets t1 + double_num_lets t2 + S (double_num_lets t1 + double_num_lets t2 + 0)); inversions H.
-    destruct t1; inversions H2; try solve [inversions H0].
-    destruct n; inversions H1. inversions H0.
+  destruct t1; inversions H2; try solve [inversions H0].
+  destruct n; inversions H1. inversions H0.
 Qed.
